well-bracketed decisions

Owl/Dist.v
@@ -192,6 +192,65 @@ Proof.
   destruct x.
   - apply H0.
   - apply H.
+Qed.
+
+Fixpoint uniform_bind_core {A B}
+         (c : Dist A) (k : A -> option (Dist B)) : option (Dist B) :=
+  match c with
+  | Ret x => k x
+  | Flip f =>
+      match uniform_bind_core (f false) k,
+            uniform_bind_core (f true)  k with
+      | Some d1, Some d2 => Some (Flip (fun b => if b then d2 else d1))
+      | _, _ => None
+      end
+  end.
+
+Definition uniform_bind {A B}
+           (co : option (Dist A)) (k : A -> option (Dist B)) : option (Dist B) :=
+  match co with
+  | None => None
+  | Some c => uniform_bind_core c k
+  end.
+
+Definition inSupportUniform {A} (c : option (Dist A)) (x : A) :=
+  match c with 
+  | None => False
+  | Some c' => (inSupport c' x) end.
+
+Lemma uniform_bind_ext_on {A B}
+  (d : option (Dist A)) (K1 K2 : A -> option (Dist B)) :
+  (forall x, inSupportUniform d x -> K1 x = K2 x) ->
+  uniform_bind d K1 = uniform_bind d K2.
+Proof.
+  intros. destruct d.
+  induction d.
+  - simpl. specialize (H a).
+    simpl in H. apply H. reflexivity.
+  - simpl in H. specialize (H0 false) as Hf. specialize (H0 true) as Ht. simpl.
+    specialize (Hf (fun x hx => H x (or_introl hx))) as Ef1. (* VERY USEFUL TOOLS *)
+    specialize (Ht (fun x hx => H x (or_intror hx))) as Et1.
+    unfold uniform_bind in Ef1. unfold uniform_bind in Et1.
+    rewrite Ef1. rewrite Et1. reflexivity.
+  - simpl. reflexivity.
+Qed.
+
+Lemma uniform_bind_all_some {A B} (c : option (Dist A)) (k : A -> option (Dist B)) d' :
+  uniform_bind c k = Some d' ->
+  forall x, inSupportUniform c x -> exists d'', k x = Some d''.
+Proof.
+  revert k d'.
+  destruct c.
+  induction d; intros k d' Hb x Hsup; simpl in *.
+  - subst. eexists. exact Hb.
+  - destruct (uniform_bind_core (d false) k) eqn:Hf0;
+    destruct (uniform_bind_core (d true)  k) eqn:Hf1;
+    try discriminate Hb.
+    inversion Hb; subst; clear Hb.
+    destruct Hsup.
+    + eapply H. apply Hf0. assumption.
+    + eapply H. apply Hf1. assumption.
+  - intros. simpl. inversion H0; subst.
 Qed. 
 
 Definition coupling {A} {B} (R : A -> B -> Prop) (d1 : Dist A) (d2 : Dist B) :=
@@ -261,7 +320,7 @@ Proof.
   reflexivity.
 Qed.
 
-Fixpoint dbind {A B} (c : Dist A) (k : forall x, inSupport c x -> Dist B) : Dist B.
+Definition dbind {A B} (c : Dist A) (k : forall x, inSupport c x -> Dist B) : Dist B.
   destruct c.
   simpl in k.
   apply (k a eq_refl).
@@ -271,7 +330,6 @@ Fixpoint dbind {A B} (c : Dist A) (k : forall x, inSupport c x -> Dist B) : Dist
   right; apply h.
   left; apply h.
 Defined.
-
 
 Lemma coupling_bind {A B C D} (d1 : Dist A) (d2 : Dist B) (k1 : A -> Dist C) (k2 : B -> Dist D) r1 r2 : 
   coupling r1 d1 d2 ->
@@ -297,55 +355,6 @@ Admitted.
   |= (x <- c1 ;; k1 x) ~ (y <- c2 ;; k2 x) { Q }.
 *)
 
-Fixpoint uniform_bind_core {A B}
-         (c : Dist A) (k : A -> option (Dist B)) : option (Dist B) :=
-  match c with
-  | Ret x => k x
-  | Flip f =>
-      match uniform_bind_core (f false) k,
-            uniform_bind_core (f true)  k with
-      | Some d1, Some d2 => Some (Flip (fun b => if b then d2 else d1))
-      | _, _ => None
-      end
-  end.
 
-Definition uniform_bind {A B}
-           (co : option (Dist A)) (k : A -> option (Dist B)) : option (Dist B) :=
-  match co with
-  | None => None
-  | Some c => uniform_bind_core c k
-  end.
-
-Lemma uniform_bind_ext_on {A B}
-  (d : Dist A) (K1 K2 : A -> option (Dist B)) :
-  (forall x, inSupport d x -> K1 x = K2 x) ->
-  uniform_bind (Some d) K1 = uniform_bind (Some d) K2.
-Proof.
-  intros.
-  induction d.
-  - simpl. specialize (H a).
-    simpl in H. apply H. reflexivity.
-  - simpl in H. specialize (H0 false) as Hf. specialize (H0 true) as Ht. simpl.
-    specialize (Hf (fun x hx => H x (or_introl hx))) as Ef1. (* VERY USEFUL TOOLS *)
-    specialize (Ht (fun x hx => H x (or_intror hx))) as Et1.
-    unfold uniform_bind in Ef1. unfold uniform_bind in Et1.
-    rewrite Ef1. rewrite Et1. reflexivity.
-Qed.
-
-Lemma uniform_bind_all_some {A B} (c : Dist A) (k : A -> option (Dist B)) d' :
-  uniform_bind (Some c) k = Some d' ->
-  forall x, inSupport c x -> exists d'', k x = Some d''.
-Proof.
-  revert k d'.
-  induction c; intros k d' Hb x Hsup; simpl in *.
-  - subst. eexists. exact Hb.
-  - destruct (uniform_bind_core (d false) k) eqn:Hf0;
-    destruct (uniform_bind_core (d true)  k) eqn:Hf1;
-    try discriminate Hb.
-    inversion Hb; subst; clear Hb.
-    destruct Hsup.
-    + eapply H. apply Hf0. assumption.
-    + eapply H. apply Hf1. assumption.
-Qed. 
 
 
